pulse/lib/pulse/core/PulseCore.Heap2.fst
@@ -15,9 +15,6 @@ let concrete h = h.concrete
 let ghost h = h.ghost
 let empty_heap = { concrete = H.empty_heap; ghost = H.empty_heap }
 
-type tag =
-  | CONCRETE
-  | GHOST
 let get (t:tag) (h:heap u#a) : GTot (H.heap u#a) =
   match t with
   | CONCRETE -> h.concrete
@@ -26,44 +23,6 @@ let put (t:tag) (h':H.heap u#a) (h:heap u#a) : GTot (heap u#a) =
   match t with
   | CONCRETE -> { h with concrete = h' }
   | GHOST -> { h with ghost = h' }
-noeq
-type splittable (a:Type) = {
-  disjoint : a -> a -> prop;
-  join : x:a -> y:a {disjoint x y } -> a;
-  laws : squash (
-    (forall (x:a) (y:a). disjoint x y <==> disjoint y x) /\
-    (forall (x:a) (y:a) (z:a). disjoint y z /\ disjoint x (join y z) ==>
-      disjoint x y /\
-      disjoint x z /\
-      disjoint (join x y) z /\
-      disjoint (join x z) y /\
-      join x (join y z) == join (join x y) z)
-  )  
-}
-noeq
-type lens (a:Type) (b:Type) = {
-  get : a -> GTot b;
-  put : b -> a -> GTot a;
-  sa: splittable a;
-  sb: splittable b;
-  lens_laws : squash (
-      (forall (x:a). put (get x) x == x) /\
-      (forall (x:a) (y:b). get (put y x) == y) /\
-      (forall (x:a) (y:b) (z:b). put z (put y x) == put z x
-    )
-  );
-  law0: (x:a) -> (y:a) -> Lemma (
-      sa.disjoint x y ==>
-      sb.disjoint (get x) (get y) /\
-      get (sa.join x y) == sb.join (get x) (get y)
-  );
-  law1: (x:a) -> (y:a) -> l:b -> m:b -> Lemma (
-        sa.disjoint x y /\
-        sb.disjoint l m ==>
-        sa.disjoint (put l x) (put m y) /\
-        sa.join (put l x) (put m y) == put (sb.join l m) (sa.join x y)
-      )
-}
 
 let core_ref = H.core_ref
 let core_ref_null = H.core_ref_null
@@ -111,57 +70,43 @@ let join_associative2 (m0 m1 m2:heap)
     join_commutative m2 m1;
     join_associative m0 m1 m2
 
-let splittable_heap : splittable (heap u#a) = {
-  disjoint;
-  join;
-  laws = FStar.Classical.forall_intro_3 disjoint_join
-}
-let splittable_hheap : splittable (H.heap u#a) = {
-  disjoint = H.disjoint;
-  join = H.join;
-  laws = admit()
-}
-let lens_concrete : lens (heap u#a) (H.heap u#a) = {
-  get = (fun h -> h.concrete);
-  put = (fun concrete h -> { h with concrete });
-  sa = splittable_heap;
-  sb = splittable_hheap;
-  lens_laws = ();
-  law0 = (fun x y -> ());
-  law1 = (fun x y l m -> ())
-}
-let lens_ghost : lens (heap u#a) (H.heap u#a) = {
-  get = (fun h -> reveal h.ghost);
-  put = (fun ghost h -> { h with ghost });
-  sa = splittable_heap;
-  sb = splittable_hheap;
-  lens_laws = ();
-  law0 = (fun x y -> ());
-  law1 = (fun x y l m -> ())
-}
-
-
+// let splittable_heap : splittable (heap u#a) = {
+//   disjoint;
+//   join;
+//   laws = FStar.Classical.forall_intro_3 disjoint_join
+// }
+// let splittable_hheap : splittable (H.heap u#a) = {
+//   disjoint = H.disjoint;
+//   join = H.join;
+//   laws = admit()
+// }
+// let lens_concrete : lens (heap u#a) (H.heap u#a) = {
+//   get = (fun h -> h.concrete);
+//   put = (fun concrete h -> { h with concrete });
+//   sa = splittable_heap;
+//   sb = splittable_hheap;
+//   lens_laws = ();
+//   law0 = (fun x y -> ());
+//   law1 = (fun x y l m -> ())
+// }
+// let lens_ghost : lens (heap u#a) (H.heap u#a) = {
+//   get = (fun h -> reveal h.ghost);
+//   put = (fun ghost h -> { h with ghost });
+//   sa = splittable_heap;
+//   sb = splittable_hheap;
+//   lens_laws = ();
+//   law0 = (fun x y -> ());
+//   law1 = (fun x y l m -> ())
+// }
 
 let slprop = p:(heap ^-> prop) { heap_prop_is_affine p }
 let interp p m = p m
 let as_slprop f = F.on _ f
 let slprop_extensionality p q = FStar.PredicateExtensionality.predicateExtensionality _ p q
 let emp = as_slprop (fun _ -> True)
-let hlens : Type u#(a + 1) = h:lens (heap u#a) (H.heap u#a) { h.sa == splittable_heap /\ h.sb == splittable_hheap }
-let llift (l:hlens) (p:H.slprop) : slprop =
-  let f : heap -> prop = (fun h -> H.of_slprop p (l.get h)) in
-  introduce forall h0 h1. f h0 /\ disjoint h0 h1 ==> f (join h0 h1)
-  with ( 
-    introduce _ ==> _
-    with _ . (
-      l.law0 h0 h1;
-      assert (l.get h0 `l.sb.disjoint` l.get h1);
-      assert (l.get (join h0 h1) == l.sb.join (l.get h0) (l.get h1))
-    )
-  );
-  as_slprop f
-let lift (p:H.slprop) : slprop = llift lens_concrete p
-  // as_slprop (fun h -> H.of_slprop p h.concrete)
+let llift (t:tag) (p:H.slprop) : slprop =
+  as_slprop (fun h -> H.of_slprop p (get t h))
+let lift (p:H.slprop) : slprop = llift CONCRETE p
 let pts_to #a #pcm (r:ref a pcm) (v:a) = lift (H.pts_to #a #pcm r v)
 let star p1 p2 =
   as_slprop (fun (h: heap) ->
@@ -190,7 +135,7 @@ let elim_h_exists #a p h = ()
 let interp_depends_only_on hp = ()
 #restart-solver
 #push-options "--fuel 0 --ifuel 2 --z3rlimit_factor 4 --split_queries always"
-let lift_star (l:hlens) (p q:H.slprop)
+let lift_star (l:tag) (p q:H.slprop)
 : Lemma (llift l (p `H.star` q) == (llift l p `star` llift l q))
         [SMTPat (llift l (p `H.star` q))]
 = introduce forall m.
@@ -208,45 +153,24 @@ let lift_star (l:hlens) (p q:H.slprop)
         interp (llift l q) h1
       returns interp (llift l (p `H.star` q)) m
       with _ . (
-        l.law0 h0 h1;
-        H.intro_star p q (l.get h0) (l.get h1)
+        H.intro_star p q (get l h0) (get l h1)
       )
     );
     introduce 
       interp (llift l (p `H.star` q)) m ==>
       interp (llift l p `star` llift l q) m
     with _ . ( 
-      H.elim_star p q (l.get m);
+      H.elim_star p q (get l m);
       eliminate exists c0 c1.
         H.disjoint c0 c1 /\
-        l.get m == H.join c0 c1 /\
+        get l m == H.join c0 c1 /\
         H.interp p c0 /\
         H.interp q c1
       returns interp (llift l p `star` llift l q) m
       with _ . (
-        let h0 = l.put c0 m in
-        let h1 = l.put c1 empty_heap in
-        l.law0 m empty_heap;
-        l.law1 m empty_heap c0 c1;
+        let h0 = put l c0 m in
+        let h1 = put l c1 empty_heap in
         assert (join h0 h1 == m)
-        //admit()
-        // introduce exists (m0 m1:heap).
-        //   disjoint m0 m1 /\
-        //   m == join m0 m1 /\
-        //   interp (llift l p) m0 /\
-        //   interp (llift l q) m1
-        // with h0 h1
-        // and (
-        //   l.laws m empty_heap 
-        // )
-
-        //   l.get m0 == c0 /\
-        //   l.get m1 == c1 /\
-        //   disjoint m0 m1
-
-        // assume (disjoint h0 h1);
-        // assume (l.get (join h0 h1) == H.join c0 c1);
-        // l.laws m empty_heap
       )
     );
     ()
@@ -259,7 +183,7 @@ let lift_emp : squash (lift H.emp == emp) =
 
 let pts_to_compatible #a #pcm (x:ref a pcm) (v0 v1:a) h = 
   H.pts_to_compatible #a #pcm x v0 v1 h.concrete;
-  lift_star lens_concrete (H.pts_to #a #pcm x v0) (H.pts_to #a #pcm x v1)
+  lift_star CONCRETE (H.pts_to #a #pcm x v0) (H.pts_to #a #pcm x v1)
 
 let pts_to_join #a #pcm (r:ref a pcm) (v1 v2:a) h =
   H.pts_to_join #a #pcm r v1 v2 h.concrete
@@ -269,7 +193,7 @@ let pts_to_join' #a #pcm r v1 v2 h =
 
 let pts_to_compatible_equiv #a #pcm r v0 v1 =
   H.pts_to_compatible_equiv #a #pcm r v0 v1;
-  lift_star lens_concrete (H.pts_to #a #pcm r v0) (H.pts_to #a #pcm r v1)
+  lift_star CONCRETE (H.pts_to #a #pcm r v0) (H.pts_to #a #pcm r v1)
 
 let pts_to_not_null #a #pcm x v m = H.pts_to_not_null #a #pcm x v m.concrete
 
@@ -293,8 +217,8 @@ let full_heap_pred h = H.full_heap_pred h.concrete /\ H.full_heap_pred h.ghost
 let heap_evolves (h0 h1:full_heap) =
   H.heap_evolves h0.concrete h1.concrete /\
   H.heap_evolves h0.ghost h1.ghost
-let free_above_addr h a = H.free_above_addr h.concrete a
-let weaken_free_above h a b = H.weaken_free_above h.concrete a b
+let free_above_addr tag h a = H.free_above_addr (get tag h) a
+let weaken_free_above tag h a b = H.weaken_free_above (get tag h) a b
 
 (** [sel_v] is a ghost read of the value contained in a heap reference *)
 let sel_v' (#a:Type u#h) (#pcm:pcm a) (r:ref a pcm) (v:erased a) (m:full_hheap (pts_to r v))
@@ -370,10 +294,10 @@ let witnessed_ref_stability #a #pcm r fact =
     )
   )
 
-let lift_pred (pre:H.full_heap -> prop)
-  : full_heap -> prop
-  = fun h -> pre h.concrete
-
+let llift_pred (l:tag) (pre:H.heap -> prop)
+  : heap -> prop
+  = fun h -> pre (get l h)
+let lift_pred = llift_pred CONCRETE
 let lift_heap_pre_action
       (#pre #post:_) (#fp:H.slprop) (#a:Type) (#fp':a -> H.slprop)
       (act:H.pre_action #pre #post fp a fp')
@@ -387,14 +311,16 @@ let lift_heap_pre_action
 
 #push-options "--fuel 0 --ifuel 0 --z3rlimit_factor 4"
 let lift_immut (m:bool) = if m then IMMUTABLE else MUTABLE
+let lift_allocs (m:bool) = if m then Some CONCRETE else None
 let lift_action
       (#immut #allocs #pre #post:_)
       (#fp:H.slprop) (#a:Type) (#fp':a -> H.slprop)
       (act:H.action #immut #allocs #pre #post fp a fp')
-: action #(lift_immut immut) #allocs #(lift_pred pre) #(lift_pred post)
+: action #(lift_immut immut) #(lift_allocs allocs) #(lift_pred pre) #(lift_pred post)
         (lift fp) a (fun x -> lift (fp' x))
 = let p = lift_heap_pre_action act in
   let mut = lift_immut immut in
+  let allocs = lift_allocs allocs in
   introduce forall frame (h0:full_hheap (lift fp `star` frame) { lift_pred pre h0 }).
     let (| x, h1 |) = p h0 in
     interp (lift (fp' x) `star` frame) h1 /\
@@ -467,9 +393,9 @@ let gather_action #a #p r v0 v1 = lift_action (H.gather_action #a #p r v0 v1)
 let pts_to_not_null_action #a #p r v = lift_action (H.pts_to_not_null_action #a #p r v)
 let extend #a #pcm x addr = lift_action (H.extend #a #pcm x addr)
 
-let refined_pre_action (#mut:mutability) (#allocates:bool)
-                       (#[T.exact (`trivial_pre)]pre:full_heap ->prop)
-                       (#[T.exact (`trivial_pre)]post:full_heap -> prop)
+let refined_pre_action (#mut:mutability) (#allocates:option tag)
+                       (#[T.exact (`trivial_pre)]pre:heap ->prop)
+                       (#[T.exact (`trivial_pre)]post:heap -> prop)
                        (fp0:slprop) (a:Type) (fp1:a -> slprop) =
   m0:full_hheap fp0 ->
   Pure (x:a &
@@ -587,6 +513,7 @@ let drop p
   refined_pre_action_as_action f
 
 let is_frame_preserving_only_ghost 
+    (#allocs:option tag)
     (#a: Type u#a)
     (#pre #post:_)
     (#fp: slprop u#b)
@@ -594,7 +521,7 @@ let is_frame_preserving_only_ghost
     (f:pre_action #pre #post fp a fp')
     (h:full_hheap fp { pre h })
 : Lemma 
-  (requires is_frame_preserving ONLY_GHOST false f)
+  (requires is_frame_preserving ONLY_GHOST allocs f)
   (ensures (dsnd (f h)).concrete == h.concrete)
 = emp_unit fp;
   let h : full_hheap (fp `star` emp) = h in
@@ -603,23 +530,21 @@ let is_frame_preserving_only_ghost
       (dsnd (f h0)).concrete == h0.concrete)
   with emp h
 
-    
-
 let lift_erased
           (#a:Type)
           (#ni_a:non_informative a)
+          (#allocs:option tag)
            #hpre #hpost
           (#pre:slprop)
           (#post:a -> slprop)
-          (frame:slprop)
-          ($f:erased (action #ONLY_GHOST #hpre #hpost pre a post))
-: action #ONLY_GHOST #hpre #hpost pre a post
-= let g : refined_pre_action #ONLY_GHOST #hpre #hpost pre a post =
+          ($f:erased (action #ONLY_GHOST #allocs #hpre #hpost pre a post))
+: action #ONLY_GHOST #allocs #hpre #hpost pre a post
+= let g : refined_pre_action #ONLY_GHOST #allocs #hpre #hpost pre a post =
     fun h ->
       let gg : erased (a & H.heap) =
-        let ff : action #ONLY_GHOST #hpre #hpost pre a post = reveal f in
+        let ff : action #ONLY_GHOST #allocs #hpre #hpost pre a post = reveal f in
         let (| x, hh' |) = ff h in
-        is_frame_preserving_only_ghost ff h;
+        is_frame_preserving_only_ghost #allocs ff h;
         Ghost.hide (x, Ghost.reveal hh'.ghost)
       in
       let x = ni_a (Ghost.hide (fst gg)) in
@@ -629,6 +554,175 @@ let lift_erased
   refined_pre_action_as_action g
 
 let ghost_ref #a p = erased H.core_ref
-let lift_ghost (p:H.slprop) : slprop = as_slprop (fun h -> H.of_slprop p h.ghost)
-let ghost_pts_to #a #p r v = lift_ghost (H.pts_to #a #p r v)
+let ghost_pts_to #a #p r v = llift GHOST (H.pts_to #a #p r v)
 let ghost_free_above_addr h addr = H.free_above_addr h.ghost addr
+
+
+let lift_heap_pre_action_ghost
+      (#pre #post:_) (#fp:H.slprop) (#a:Type) (#fp':a -> H.slprop)
+      (ni_a:non_informative a)
+      (act:H.pre_action #pre #post fp a fp')
+: pre_action #(llift_pred GHOST pre) #(llift_pred GHOST post)
+              (llift GHOST fp)
+              a
+              (fun x -> llift GHOST (fp' x))
+= fun (h0:full_hheap (llift GHOST fp) { llift_pred GHOST pre h0 }) ->
+    let xg : erased (a & H.heap) = 
+      let (| x, g |) = act (reveal h0.ghost) in
+      hide (x, g)
+    in
+    let h1 = { h0 with ghost=hide (snd (reveal xg)) } in
+    let x = ni_a (hide (fst (reveal xg))) in
+    (| x, h1 |)
+
+#restart-solver
+
+#push-options "--fuel 0 --ifuel 0 --z3rlimit_factor 4"
+let lift_immut_ghost (m:bool) = if m then IMMUTABLE else ONLY_GHOST
+let lift_allocs_ghost (m:bool) = if m then Some GHOST else None
+let lift_action_ghost
+      (#immut #allocs #pre #post:_)
+      (#fp:H.slprop) (#a:Type) (#fp':a -> H.slprop)
+      (ni_a:non_informative a)
+      (act:H.action #immut #allocs #pre #post fp a fp')
+: action #(lift_immut_ghost immut)
+         #(lift_allocs_ghost allocs)
+         #(llift_pred GHOST pre) #(llift_pred GHOST post)
+         (llift GHOST fp) a (fun x -> llift GHOST (fp' x))
+= let p = lift_heap_pre_action_ghost ni_a act in
+  let mut = lift_immut immut in
+  let allocs = lift_allocs_ghost allocs in
+  introduce forall frame (h0:full_hheap (llift GHOST fp `star` frame) { llift_pred GHOST pre h0 }).
+    let (| x, h1 |) = p h0 in
+    interp (llift GHOST (fp' x) `star` frame) h1 /\
+    action_related_heaps #mut #allocs h0 h1
+  with (
+    assert (interp (llift GHOST fp `star` frame) h0);
+    let (| x, h1 |) = p h0 in
+    eliminate exists h0' h1'.
+      disjoint h0' h1' /\
+      h0 == join h0' h1' /\
+      interp (llift GHOST fp) h0' /\
+      interp frame h1'
+    returns 
+      interp (llift GHOST (fp' x) `star` frame) h1 /\
+      action_related_heaps #mut #allocs h0 h1
+    with _ . (
+      let hframe : H.heap -> prop = (fun h -> interp frame { concrete = h1'.concrete; ghost = h }) in
+      introduce forall c0 c1.
+        (hframe c0 /\ H.disjoint c0 c1)
+         ==> 
+        hframe (H.join c0 c1)
+      with (
+        introduce _ ==> _
+        with _ . (
+          let h0g = {concrete=h1'.concrete; ghost=c0 } in
+          assert (interp frame h0g);
+          assert (H.disjoint c0 c1);
+          assert (heap_prop_is_affine frame);
+          let h1g = { concrete = H.empty_heap; ghost=c1} in
+          assert (disjoint h0g h1g);
+          assert (interp frame (join h0g h1g));
+          assert (hframe (H.join c0 c1))
+        )
+      );
+      assert (H.heap_prop_is_affine hframe);
+      let hframe : H.slprop = H.as_slprop hframe in
+      assert (H.interp fp h0'.ghost);
+      assert (H.interp hframe h1'.ghost);
+      H.intro_star fp hframe h0'.ghost h1'.ghost;
+      let h00 : H.full_hheap (fp `H.star` hframe) = h0.ghost in
+      let h11 : H.full_hheap (fp' x `H.star` hframe) = dsnd (act h00) in
+      assert (h1 == { h0 with ghost = h11 });
+      H.elim_star (fp' x) hframe h11;
+      eliminate exists c0 c1.
+        H.disjoint c0 c1 /\
+        h11 == H.join c0 c1 /\
+        H.interp (fp' x) c0 /\
+        H.interp hframe c1
+      returns interp (llift GHOST (fp' x) `star` frame) h1
+      with _ . ( 
+        let h10 = { concrete = h0'.concrete; ghost=c0 } in
+        let h11 = { concrete = h1'.concrete; ghost=c1 } in
+        assert (interp (llift GHOST (fp' x)) h10);
+        assert (interp frame h11);
+        assert (disjoint h10 h11)
+      );
+      heap_evolves_iff h0 h1;
+      assert (action_related_heaps #mut #allocs h0 h1)
+    )
+  );
+  p
+
+let ni_erased a : non_informative (erased a) = fun x -> reveal x
+let ni_unit : non_informative unit = fun x -> reveal x
+
+let lift_ghost_emp : squash (llift GHOST H.emp == emp) = 
+  FStar.Classical.forall_intro H.intro_emp;
+  slprop_extensionality (llift GHOST H.emp) emp
+let ghost_extend
+    (#a:Type u#a)
+    (#pcm:pcm a)
+    (x:erased a{compatible pcm x x /\ pcm.refine x})
+    (addr:erased nat)
+= lift_erased #_ #(ni_erased H.core_ref)
+    (Ghost.hide <|
+      lift_action_ghost (ni_erased H.core_ref) (H.erase_action_result (H.extend #a #pcm x addr)))
+
+
+let ghost_read
+    (#a:Type)
+    (#p:pcm a)
+    (r:ghost_ref p)
+    (x:erased a)
+    (f:(v:a{compatible p x v}
+        -> GTot (y:a{compatible p y v /\
+                     FStar.PCM.frame_compatible p x v y})))
+= lift_erased #_ #(ni_erased _) #None
+    (Ghost.hide <|
+      lift_action_ghost (ni_erased _) (H.erase_action_result (H.select_refine #a #p r x f)))
+
+let ghost_write
+    (#a:Type)
+    (#p:pcm a)
+    (r:ghost_ref p)
+    (x y:Ghost.erased a)
+    (f:FStar.PCM.frame_preserving_upd p x y)
+: action #ONLY_GHOST #None
+    (ghost_pts_to r x)
+    unit
+    (fun _ -> ghost_pts_to r y)
+= lift_erased #_ #(ni_unit) #None
+    (Ghost.hide <|
+      lift_action_ghost ni_unit (H.upd_gen_action #a #p r x y f))
+
+
+let ghost_share
+    (#a:Type)
+    (#pcm:pcm a)
+    (r:ghost_ref pcm)
+    (v0:FStar.Ghost.erased a)
+    (v1:FStar.Ghost.erased a{composable pcm v0 v1})
+: action #IMMUTABLE
+    (ghost_pts_to r (v0 `op pcm` v1))
+    unit
+    (fun _ -> ghost_pts_to r v0 `star` ghost_pts_to r v1)
+= lift_erased #_ #(ni_unit) #None
+    (Ghost.hide <|
+      lift_action_ghost ni_unit (H.split_action #a #pcm r v0 v1))
+
+let ni_squash #a : non_informative (squash a) = fun x -> reveal x
+
+let ghost_gather
+    (#a:Type)
+    (#pcm:pcm a)
+    (r:ghost_ref pcm)
+    (v0:FStar.Ghost.erased a)
+    (v1:FStar.Ghost.erased a)
+: action #IMMUTABLE 
+    (ghost_pts_to r v0 `star` ghost_pts_to r v1)
+    (squash (composable pcm v0 v1))
+    (fun _ -> ghost_pts_to r (op pcm v0 v1))
+= lift_erased #_ #(ni_squash ) #None
+    (Ghost.hide <|
+      lift_action_ghost ni_squash (H.gather_action #a #pcm r v0 v1))
